alignment to an usual redblack (oiwiki)

vfa/redblack.ml
@@ -21,6 +21,12 @@ let rec lookup d x = function
 | T (_, tl, k, v, tr) ->
   if ( < ) x k then lookup d x tl else if ( < ) k x then lookup d x tr else v
 
+(** val make_black : 'a1 tree -> 'a1 tree **)
+
+let make_black = function
+| E -> E
+| T (_, a, x, vx, b) -> T (Black, a, x, vx, b)
+
 (** val balance : color -> 'a1 tree -> key -> 'a1 -> 'a1 tree -> 'a1 tree **)
 
 let balance c t1 k vk t2 =
@@ -41,22 +47,50 @@ let balance c t1 k vk t2 =
                  | T (c1, c2, z, vz, d0) ->
                    (match c1 with
                     | Red ->
-                      T (Red, (T (Black, t1, k, vk, b)), y, vy, (T (Black,
-                        c2, z, vz, d0)))
+                      (match t1 with
+                       | E ->
+                         T (Black, (T (Red, t1, k, vk, b)), y, vy, (T (Red,
+                           c2, z, vz, d0)))
+                       | T (c3, _, _, _, _) ->
+                         (match c3 with
+                          | Red ->
+                            T (Red, (make_black t1), k, vk, (make_black t2))
+                          | Black ->
+                            T (Black, (T (Red, t1, k, vk, b)), y, vy, (T
+                              (Red, c2, z, vz, d0)))))
                     | Black -> T (Black, t1, k, vk, t2)))
               | T (c1, b0, y0, vy0, c2) ->
                 (match c1 with
                  | Red ->
-                   T (Red, (T (Black, t1, k, vk, b0)), y0, vy0, (T (Black,
-                     c2, y, vy, d)))
+                   (match t1 with
+                    | E ->
+                      T (Black, (T (Red, t1, k, vk, b0)), y0, vy0, (T (Red,
+                        c2, y, vy, d)))
+                    | T (c3, _, _, _, _) ->
+                      (match c3 with
+                       | Red ->
+                         T (Red, (make_black t1), k, vk, (make_black t2))
+                       | Black ->
+                         T (Black, (T (Red, t1, k, vk, b0)), y0, vy0, (T
+                           (Red, c2, y, vy, d)))))
                  | Black ->
                    (match d with
                     | E -> T (Black, t1, k, vk, t2)
                     | T (c3, c4, z, vz, d0) ->
                       (match c3 with
                        | Red ->
-                         T (Red, (T (Black, t1, k, vk, b)), y, vy, (T (Black,
-                           c4, z, vz, d0)))
+                         (match t1 with
+                          | E ->
+                            T (Black, (T (Red, t1, k, vk, b)), y, vy, (T
+                              (Red, c4, z, vz, d0)))
+                          | T (c5, _, _, _, _) ->
+                            (match c5 with
+                             | Red ->
+                               T (Red, (make_black t1), k, vk,
+                                 (make_black t2))
+                             | Black ->
+                               T (Black, (T (Red, t1, k, vk, b)), y, vy, (T
+                                 (Red, c4, z, vz, d0)))))
                        | Black -> T (Black, t1, k, vk, t2)))))
            | Black -> T (Black, t1, k, vk, t2)))
      | T (c0, a, x, vx, c1) ->
@@ -78,29 +112,68 @@ let balance c t1 k vk t2 =
                           | T (c3, c4, z, vz, d0) ->
                             (match c3 with
                              | Red ->
-                               T (Red, (T (Black, t1, k, vk, b)), y, vy, (T
-                                 (Black, c4, z, vz, d0)))
+                               (match t1 with
+                                | E ->
+                                  T (Black, (T (Red, t1, k, vk, b)), y, vy,
+                                    (T (Red, c4, z, vz, d0)))
+                                | T (c5, _, _, _, _) ->
+                                  (match c5 with
+                                   | Red ->
+                                     T (Red, (make_black t1), k, vk,
+                                       (make_black t2))
+                                   | Black ->
+                                     T (Black, (T (Red, t1, k, vk, b)), y,
+                                       vy, (T (Red, c4, z, vz, d0)))))
                              | Black -> T (Black, t1, k, vk, t2)))
                        | T (c3, b0, y0, vy0, c4) ->
                          (match c3 with
                           | Red ->
-                            T (Red, (T (Black, t1, k, vk, b0)), y0, vy0, (T
-                              (Black, c4, y, vy, d)))
+                            (match t1 with
+                             | E ->
+                               T (Black, (T (Red, t1, k, vk, b0)), y0, vy0,
+                                 (T (Red, c4, y, vy, d)))
+                             | T (c5, _, _, _, _) ->
+                               (match c5 with
+                                | Red ->
+                                  T (Red, (make_black t1), k, vk,
+                                    (make_black t2))
+                                | Black ->
+                                  T (Black, (T (Red, t1, k, vk, b0)), y0,
+                                    vy0, (T (Red, c4, y, vy, d)))))
                           | Black ->
                             (match d with
                              | E -> T (Black, t1, k, vk, t2)
                              | T (c5, c6, z, vz, d0) ->
                                (match c5 with
                                 | Red ->
-                                  T (Red, (T (Black, t1, k, vk, b)), y, vy,
-                                    (T (Black, c6, z, vz, d0)))
+                                  (match t1 with
+                                   | E ->
+                                     T (Black, (T (Red, t1, k, vk, b)), y,
+                                       vy, (T (Red, c6, z, vz, d0)))
+                                   | T (c7, _, _, _, _) ->
+                                     (match c7 with
+                                      | Red ->
+                                        T (Red, (make_black t1), k, vk,
+                                          (make_black t2))
+                                      | Black ->
+                                        T (Black, (T (Red, t1, k, vk, b)), y,
+                                          vy, (T (Red, c6, z, vz, d0)))))
                                 | Black -> T (Black, t1, k, vk, t2)))))
                     | Black -> T (Black, t1, k, vk, t2)))
               | T (c2, b, y, vy, c3) ->
                 (match c2 with
                  | Red ->
-                   T (Red, (T (Black, a, x, vx, b)), y, vy, (T (Black, c3, k,
-                     vk, t2)))
+                   (match t2 with
+                    | E ->
+                      T (Black, (T (Red, a, x, vx, b)), y, vy, (T (Red, c3,
+                        k, vk, t2)))
+                    | T (c4, _, _, _, _) ->
+                      (match c4 with
+                       | Red ->
+                         T (Red, (make_black t1), k, vk, (make_black t2))
+                       | Black ->
+                         T (Black, (T (Red, a, x, vx, b)), y, vy, (T (Red,
+                           c3, k, vk, t2)))))
                  | Black ->
                    (match t2 with
                     | E -> T (Black, t1, k, vk, t2)
@@ -114,29 +187,68 @@ let balance c t1 k vk t2 =
                              | T (c5, c6, z, vz, d0) ->
                                (match c5 with
                                 | Red ->
-                                  T (Red, (T (Black, t1, k, vk, b0)), y0,
-                                    vy0, (T (Black, c6, z, vz, d0)))
+                                  (match t1 with
+                                   | E ->
+                                     T (Black, (T (Red, t1, k, vk, b0)), y0,
+                                       vy0, (T (Red, c6, z, vz, d0)))
+                                   | T (c7, _, _, _, _) ->
+                                     (match c7 with
+                                      | Red ->
+                                        T (Red, (make_black t1), k, vk,
+                                          (make_black t2))
+                                      | Black ->
+                                        T (Black, (T (Red, t1, k, vk, b0)),
+                                          y0, vy0, (T (Red, c6, z, vz, d0)))))
                                 | Black -> T (Black, t1, k, vk, t2)))
                           | T (c5, b1, y1, vy1, c6) ->
                             (match c5 with
                              | Red ->
-                               T (Red, (T (Black, t1, k, vk, b1)), y1, vy1,
-                                 (T (Black, c6, y0, vy0, d)))
+                               (match t1 with
+                                | E ->
+                                  T (Black, (T (Red, t1, k, vk, b1)), y1,
+                                    vy1, (T (Red, c6, y0, vy0, d)))
+                                | T (c7, _, _, _, _) ->
+                                  (match c7 with
+                                   | Red ->
+                                     T (Red, (make_black t1), k, vk,
+                                       (make_black t2))
+                                   | Black ->
+                                     T (Black, (T (Red, t1, k, vk, b1)), y1,
+                                       vy1, (T (Red, c6, y0, vy0, d)))))
                              | Black ->
                                (match d with
                                 | E -> T (Black, t1, k, vk, t2)
                                 | T (c7, c8, z, vz, d0) ->
                                   (match c7 with
                                    | Red ->
-                                     T (Red, (T (Black, t1, k, vk, b0)), y0,
-                                       vy0, (T (Black, c8, z, vz, d0)))
+                                     (match t1 with
+                                      | E ->
+                                        T (Black, (T (Red, t1, k, vk, b0)),
+                                          y0, vy0, (T (Red, c8, z, vz, d0)))
+                                      | T (c9, _, _, _, _) ->
+                                        (match c9 with
+                                         | Red ->
+                                           T (Red, (make_black t1), k, vk,
+                                             (make_black t2))
+                                         | Black ->
+                                           T (Black, (T (Red, t1, k, vk,
+                                             b0)), y0, vy0, (T (Red, c8, z,
+                                             vz, d0)))))
                                    | Black -> T (Black, t1, k, vk, t2)))))
                        | Black -> T (Black, t1, k, vk, t2)))))
            | T (c2, a0, x0, vx0, b) ->
              (match c2 with
               | Red ->
-                T (Red, (T (Black, a0, x0, vx0, b)), x, vx, (T (Black, c1, k,
-                  vk, t2)))
+                (match t2 with
+                 | E ->
+                   T (Black, (T (Red, a0, x0, vx0, b)), x, vx, (T (Red, c1,
+                     k, vk, t2)))
+                 | T (c3, _, _, _, _) ->
+                   (match c3 with
+                    | Red -> T (Red, (make_black t1), k, vk, (make_black t2))
+                    | Black ->
+                      T (Black, (T (Red, a0, x0, vx0, b)), x, vx, (T (Red,
+                        c1, k, vk, t2)))))
               | Black ->
                 (match c1 with
                  | E ->
@@ -152,29 +264,69 @@ let balance c t1 k vk t2 =
                              | T (c4, c5, z, vz, d0) ->
                                (match c4 with
                                 | Red ->
-                                  T (Red, (T (Black, t1, k, vk, b0)), y, vy,
-                                    (T (Black, c5, z, vz, d0)))
+                                  (match t1 with
+                                   | E ->
+                                     T (Black, (T (Red, t1, k, vk, b0)), y,
+                                       vy, (T (Red, c5, z, vz, d0)))
+                                   | T (c6, _, _, _, _) ->
+                                     (match c6 with
+                                      | Red ->
+                                        T (Red, (make_black t1), k, vk,
+                                          (make_black t2))
+                                      | Black ->
+                                        T (Black, (T (Red, t1, k, vk, b0)),
+                                          y, vy, (T (Red, c5, z, vz, d0)))))
                                 | Black -> T (Black, t1, k, vk, t2)))
                           | T (c4, b1, y0, vy0, c5) ->
                             (match c4 with
                              | Red ->
-                               T (Red, (T (Black, t1, k, vk, b1)), y0, vy0,
-                                 (T (Black, c5, y, vy, d)))
+                               (match t1 with
+                                | E ->
+                                  T (Black, (T (Red, t1, k, vk, b1)), y0,
+                                    vy0, (T (Red, c5, y, vy, d)))
+                                | T (c6, _, _, _, _) ->
+                                  (match c6 with
+                                   | Red ->
+                                     T (Red, (make_black t1), k, vk,
+                                       (make_black t2))
+                                   | Black ->
+                                     T (Black, (T (Red, t1, k, vk, b1)), y0,
+                                       vy0, (T (Red, c5, y, vy, d)))))
                              | Black ->
                                (match d with
                                 | E -> T (Black, t1, k, vk, t2)
                                 | T (c6, c7, z, vz, d0) ->
                                   (match c6 with
                                    | Red ->
-                                     T (Red, (T (Black, t1, k, vk, b0)), y,
-                                       vy, (T (Black, c7, z, vz, d0)))
+                                     (match t1 with
+                                      | E ->
+                                        T (Black, (T (Red, t1, k, vk, b0)),
+                                          y, vy, (T (Red, c7, z, vz, d0)))
+                                      | T (c8, _, _, _, _) ->
+                                        (match c8 with
+                                         | Red ->
+                                           T (Red, (make_black t1), k, vk,
+                                             (make_black t2))
+                                         | Black ->
+                                           T (Black, (T (Red, t1, k, vk,
+                                             b0)), y, vy, (T (Red, c7, z, vz,
+                                             d0)))))
                                    | Black -> T (Black, t1, k, vk, t2)))))
                        | Black -> T (Black, t1, k, vk, t2)))
                  | T (c3, b0, y, vy, c4) ->
                    (match c3 with
                     | Red ->
-                      T (Red, (T (Black, a, x, vx, b0)), y, vy, (T (Black,
-                        c4, k, vk, t2)))
+                      (match t2 with
+                       | E ->
+                         T (Black, (T (Red, a, x, vx, b0)), y, vy, (T (Red,
+                           c4, k, vk, t2)))
+                       | T (c5, _, _, _, _) ->
+                         (match c5 with
+                          | Red ->
+                            T (Red, (make_black t1), k, vk, (make_black t2))
+                          | Black ->
+                            T (Black, (T (Red, a, x, vx, b0)), y, vy, (T
+                              (Red, c4, k, vk, t2)))))
                     | Black ->
                       (match t2 with
                        | E -> T (Black, t1, k, vk, t2)
@@ -188,22 +340,55 @@ let balance c t1 k vk t2 =
                                 | T (c6, c7, z, vz, d0) ->
                                   (match c6 with
                                    | Red ->
-                                     T (Red, (T (Black, t1, k, vk, b1)), y0,
-                                       vy0, (T (Black, c7, z, vz, d0)))
+                                     (match t1 with
+                                      | E ->
+                                        T (Black, (T (Red, t1, k, vk, b1)),
+                                          y0, vy0, (T (Red, c7, z, vz, d0)))
+                                      | T (c8, _, _, _, _) ->
+                                        (match c8 with
+                                         | Red ->
+                                           T (Red, (make_black t1), k, vk,
+                                             (make_black t2))
+                                         | Black ->
+                                           T (Black, (T (Red, t1, k, vk,
+                                             b1)), y0, vy0, (T (Red, c7, z,
+                                             vz, d0)))))
                                    | Black -> T (Black, t1, k, vk, t2)))
                              | T (c6, b2, y1, vy1, c7) ->
                                (match c6 with
                                 | Red ->
-                                  T (Red, (T (Black, t1, k, vk, b2)), y1,
-                                    vy1, (T (Black, c7, y0, vy0, d)))
+                                  (match t1 with
+                                   | E ->
+                                     T (Black, (T (Red, t1, k, vk, b2)), y1,
+                                       vy1, (T (Red, c7, y0, vy0, d)))
+                                   | T (c8, _, _, _, _) ->
+                                     (match c8 with
+                                      | Red ->
+                                        T (Red, (make_black t1), k, vk,
+                                          (make_black t2))
+                                      | Black ->
+                                        T (Black, (T (Red, t1, k, vk, b2)),
+                                          y1, vy1, (T (Red, c7, y0, vy0, d)))))
                                 | Black ->
                                   (match d with
                                    | E -> T (Black, t1, k, vk, t2)
                                    | T (c8, c9, z, vz, d0) ->
                                      (match c8 with
                                       | Red ->
-                                        T (Red, (T (Black, t1, k, vk, b1)),
-                                          y0, vy0, (T (Black, c9, z, vz, d0)))
+                                        (match t1 with
+                                         | E ->
+                                           T (Black, (T (Red, t1, k, vk,
+                                             b1)), y0, vy0, (T (Red, c9, z,
+                                             vz, d0)))
+                                         | T (c10, _, _, _, _) ->
+                                           (match c10 with
+                                            | Red ->
+                                              T (Red, (make_black t1), k, vk,
+                                                (make_black t2))
+                                            | Black ->
+                                              T (Black, (T (Red, t1, k, vk,
+                                                b1)), y0, vy0, (T (Red, c9,
+                                                z, vz, d0)))))
                                       | Black -> T (Black, t1, k, vk, t2)))))
                           | Black -> T (Black, t1, k, vk, t2)))))))
         | Black ->
@@ -219,22 +404,51 @@ let balance c t1 k vk t2 =
                     | T (c3, c4, z, vz, d0) ->
                       (match c3 with
                        | Red ->
-                         T (Red, (T (Black, t1, k, vk, b)), y, vy, (T (Black,
-                           c4, z, vz, d0)))
+                         (match t1 with
+                          | E ->
+                            T (Black, (T (Red, t1, k, vk, b)), y, vy, (T
+                              (Red, c4, z, vz, d0)))
+                          | T (c5, _, _, _, _) ->
+                            (match c5 with
+                             | Red ->
+                               T (Red, (make_black t1), k, vk,
+                                 (make_black t2))
+                             | Black ->
+                               T (Black, (T (Red, t1, k, vk, b)), y, vy, (T
+                                 (Red, c4, z, vz, d0)))))
                        | Black -> T (Black, t1, k, vk, t2)))
                  | T (c3, b0, y0, vy0, c4) ->
                    (match c3 with
                     | Red ->
-                      T (Red, (T (Black, t1, k, vk, b0)), y0, vy0, (T (Black,
-                        c4, y, vy, d)))
+                      (match t1 with
+                       | E ->
+                         T (Black, (T (Red, t1, k, vk, b0)), y0, vy0, (T
+                           (Red, c4, y, vy, d)))
+                       | T (c5, _, _, _, _) ->
+                         (match c5 with
+                          | Red ->
+                            T (Red, (make_black t1), k, vk, (make_black t2))
+                          | Black ->
+                            T (Black, (T (Red, t1, k, vk, b0)), y0, vy0, (T
+                              (Red, c4, y, vy, d)))))
                     | Black ->
                       (match d with
                        | E -> T (Black, t1, k, vk, t2)
                        | T (c5, c6, z, vz, d0) ->
                          (match c5 with
                           | Red ->
-                            T (Red, (T (Black, t1, k, vk, b)), y, vy, (T
-                              (Black, c6, z, vz, d0)))
+                            (match t1 with
+                             | E ->
+                               T (Black, (T (Red, t1, k, vk, b)), y, vy, (T
+                                 (Red, c6, z, vz, d0)))
+                             | T (c7, _, _, _, _) ->
+                               (match c7 with
+                                | Red ->
+                                  T (Red, (make_black t1), k, vk,
+                                    (make_black t2))
+                                | Black ->
+                                  T (Black, (T (Red, t1, k, vk, b)), y, vy,
+                                    (T (Red, c6, z, vz, d0)))))
                           | Black -> T (Black, t1, k, vk, t2)))))
               | Black -> T (Black, t1, k, vk, t2)))))
 
@@ -246,12 +460,6 @@ let rec ins x vx = function
   if ( < ) x y
   then balance c (ins x vx a) y vy b
   else if ( < ) y x then balance c a y vy (ins x vx b) else T (c, a, x, vx, b)
-
-(** val make_black : 'a1 tree -> 'a1 tree **)
-
-let make_black = function
-| E -> E
-| T (_, a, x, vx, b) -> T (Black, a, x, vx, b)
 
 (** val insert : key -> 'a1 -> 'a1 tree -> 'a1 tree **)
 
